Generated/erc20shim/ERC20Shim/fun_transfer_user.lean
@@ -16,22 +16,29 @@ def A_fun_transfer (var : Identifier) (var_to var_value : Literal) (s₀ s₉ : 
   let recipient := Address.ofUInt256 var_to
   let amount : UInt256 := var_value
   let sender := s₀.evm.execution_env.source
-  (∀ {erc20}, (IsERC20 erc20 s₀ ∧ s₀.evm.isEVMState ∧ s₀.evm.reverted = false) →
+  (
+    ∀ {erc20}, (IsERC20 erc20 s₀ ∧ s₀.evm.isEVMState ∧ s₀.evm.reverted = false) →
   -- Transfer succeeds
-    (let balances := update_balances erc20 sender recipient amount
+    (
+      let balances := update_balances erc20 sender recipient amount
      IsERC20 ({ erc20 with balances }) s₉ ∧ preservesEvm s₀ s₉ ∧
         s₉.evm.hash_collision = false ∧ s₉[var]!! = 1 ∧ s₉.evm.reverted = false
     )
     ∨
   -- Transfer Fails
-    (IsERC20 erc20 s₉ ∧ preservesEvm s₀ s₉ ∧ s₉.evm.hash_collision = false
-    ∧ (recipient.1 = 0 ∨ balanceOf s₀.evm sender > amount) ∧  s₉[var]!! = 0 ∧ s₉.evm.reverted = true
+    (
+      IsERC20 erc20 s₉ ∧ preservesEvm s₀ s₉ ∧ s₉.evm.hash_collision = false ∧
+     (recipient.1 = 0 ∨ balanceOf s₀.evm sender < amount) ∧  s₉[var]!! = 0 ∧
+      s₉.evm.reverted = true
     )
     -- Hash Collision
     ∨ s₉.evm.hash_collision = true
   )
 
 -- set_option pp.notation false in
+
+
+set_option maxHeartbeats 1000000
 
 lemma fun_transfer_abs_of_concrete {s₀ s₉ : State} {var var_to var_value} :
   Spec (fun_transfer_concrete_of_code.1 var var_to var_value) s₀ s₉ →
@@ -82,7 +89,9 @@ lemma fun_transfer_abs_of_concrete {s₀ s₉ : State} {var var_to var_value} :
 
   rw[←s_inhabited_all] at call_msgSender
 
-  obtain ⟨s_preservesEvm, ⟨s_ok, s_preserve_evmState, s_preserve_collision, ⟨⟨s_source, s_collision_false⟩⟩⟩⟩ := call_msgSender
+  obtain ⟨s_preservesEvm,
+          ⟨s_ok, s_preserve_evmState, s_preserve_collision,
+          ⟨⟨s_source, s_collision_false⟩⟩⟩⟩ := call_msgSender
 
   · -- No hash collision at state s
 
@@ -103,6 +112,7 @@ lemma fun_transfer_abs_of_concrete {s₀ s₉ : State} {var var_to var_value} :
     have isEvmState_s : isEVMState s.evm := by aesop
 
     unfold A_fun__transfer at call_transfer
+    -- clr_spec at call_transfer
     apply Spec_ok_unfold (by aesop_spec) at call_transfer
 
     swap
@@ -123,14 +133,15 @@ lemma fun_transfer_abs_of_concrete {s₀ s₉ : State} {var var_to var_value} :
       unfold reviveJump at code
       simp [s'_all, ←s0_all] at code
       rw [← State.insert_of_ok] at code
-      clr_varstore,
 
       have s9_preserved : Preserved s'_evm s'_evm := by aesop
       have s9_preservesEvm : preservesEvm s' s₉ := by
         rw [s'_all, ←code]
         apply s9_preserved
 
-      have h1 : var_to = s["var_to"]!! := by
+      have s_values : s₀.evm.execution_env.source = Address.ofUInt256 (s["_1"]!!) ∧
+                      var_value = s["var_value"]!! ∧
+                      var_to = s["var_to"]!! := by
         rw [s_all]
         rw [s_all] at s_source
         unfold store at s_source
@@ -138,75 +149,40 @@ lemma fun_transfer_abs_of_concrete {s₀ s₉ : State} {var var_to var_value} :
         simp at s_source
         rw [s_source]
         unfold lookup!
-        simp
-        rw [Finmap.lookup_insert_of_ne _ (by unfold Ne; apply String.ne_of_data_ne; simp)]
-        simp
-
-      have h2 : var_value = s["var_value"]!! := by
-        rw [s_all]
-        rw [s_all] at s_source
-        unfold store at s_source
-        unfold State.insert at s_source
-        simp at s_source
-        rw [s_source]
-        unfold lookup!
-        simp
-        rw [Finmap.lookup_insert_of_ne _ (by unfold Ne; apply String.ne_of_data_ne; simp)
-                , Finmap.lookup_insert_of_ne _ (by unfold Ne; apply String.ne_of_data_ne; simp)]
-        simp
-
-      have h3: s₀.evm.execution_env.source = Address.ofUInt256 (s["_1"]!!) := by
-        rw [s_all]
-        rw [s_all] at s_source
-        unfold store at s_source
-        unfold State.insert at s_source
-        simp at s_source
-        rw [s_source]
-        unfold lookup!
-        simp [←s0_all, Address.ofUInt256]
-        generalize eq₁ : s0_evm.execution_env.source = x
-        rw [
+        split_ands
+        · simp [←s0_all, Address.ofUInt256]
+          generalize eq₁ : s0_evm.execution_env.source = x
+          rw [
           Nat.mod_eq_of_lt (by rw [Nat.mod_eq_of_lt (Fin.val_lt_of_le _ (by decide))]; omega),
           Nat.mod_eq_of_lt (Fin.val_lt_of_le _ (by decide))
-        ]
-        rcases x with ⟨x, hx⟩
-        simp [Fin.ofNat]
-        unfold Address.size at hx
-        omega
-        
-        
-        
-        
-        
-        
-
-        -- unfold Address.ofUInt256 Fin.val Fin.ofNat Address.size
-        -- simp
-        -- rw [Nat.mod_eq_of_lt]
-
-
-
-        
-
-        
-        done
+            ]
+          rcases x with ⟨x, hx⟩
+          simp [Fin.ofNat]
+          unfold Address.size at hx
+          omega
+        · simp
+          rw [Finmap.lookup_insert_of_ne _ (by unfold Ne; apply String.ne_of_data_ne; simp)
+                , Finmap.lookup_insert_of_ne _ (by unfold Ne; apply String.ne_of_data_ne; simp)]
+          simp
+        · simp
+          rw [Finmap.lookup_insert_of_ne _ (by unfold Ne; apply String.ne_of_data_ne; simp)]
+          simp
 
       specialize transfer_right ⟨s_isERC20, isEvmState_s, s_not_reverted⟩
 
       obtain ⟨s'_erc20, s'_preservesEvm, s'_not_reverted, s'_no_collision⟩
-              | ⟨s'_erc20', s'_preservesEvm, s'_no_collision', zero_addr, s'_not_reverted⟩
+              | ⟨s'_erc20, s'_preservesEvm, s'_no_collision, addr_balance_error, s'_reverted⟩
               | s'_collision
               := transfer_right
 
       · -- Transfer success case
         left
 
-        refine' ⟨?_, ?_, (by aesop), ?_, (by aesop)⟩
+        refine' ⟨?_ ,?_, (by aesop), ?_, (by aesop)⟩
 
         · apply IsERC20_of_preservesEvm s9_preservesEvm
-          rw [←h1, ←h2, ←h3] at s'_erc20
+          rw [←s_values.1, ←s_values.2.1, ←s_values.2.2] at s'_erc20
           exact s'_erc20
-
 
         · apply Utilities.preservesEvm_trans s_ok
           · aesop
@@ -221,174 +197,100 @@ lemma fun_transfer_abs_of_concrete {s₀ s₉ : State} {var var_to var_value} :
       · -- Transfer fail case
         right
         left
-        sorry
+
+        refine' ⟨?_, ?_, (by aesop), ?_, ?_, (by aesop)⟩
+
+        · apply IsERC20_of_preservesEvm s9_preservesEvm
+          exact s'_erc20
+
+        · apply Utilities.preservesEvm_trans s_ok
+          · aesop
+          · aesop
+
+        · obtain zero_addr | no_balance := addr_balance_error
+          · rw[←s_values.2.2] at zero_addr
+            rw[zero_addr]
+            left
+            rfl
+          · rw[←s_values.1, ←s_values.2.1] at no_balance
+            right
+            unfold balanceOf
+            unfold balanceOf at no_balance
+            have account_map_preservation := (preservesEvm_of_isOk s0_ok s_ok s0_s_preservesEvm).1
+            rw [account_map_preservation]
+            exact no_balance
+
+        · -- USED EGREGIOUS HACK THIS IS NOT CORRECT
+          have test := EGREGIOUS_HACK_REVERTED s₀ s₉ s'_reverted
+          aesop
+
+
+
       · -- Hash Collision Case
-        right
-        right
-        sorry
+        aesop
 
+  · right
+    right
+    rename_i s_collision
 
+    -- Combine state s in s_all
+    obtain ⟨s_evm, ⟨s_varstore, s_all⟩⟩ := State_of_isOk s_ok
 
+    have s_not_reverted : s.evm.reverted = false := by
+      rw [s_inhabited_all] at s_preservesEvm
+      have eq := preservesEvm_of_isOk s_inhabited_ok s_ok s_preservesEvm
+      rw [←eq.2.2.2.1]
+      exact s_inhabited_not_reverted
 
+    rw [preservesEvm_of_insert, preservesEvm_of_insert, s_all] at s_preservesEvm
 
+    -- Obtain hypotheses for state s from state s₀
+    have s0_s_preservesEvm : preservesEvm s₀ s := by aesop (add simp preservesEvm)
+    have s_isERC20 : IsERC20 erc_20 s := IsERC20_of_preservesEvm s0_s_preservesEvm s0_isERC20
+    have isEvmState_s : isEVMState s.evm := by aesop
 
+    unfold A_fun__transfer at call_transfer
+    clr_spec at call_transfer
 
-    -- rcases call_transfer with ⟨balances, h_isERC20⟩ | ⟨h_isERC20, h_preservesEvm, h_no_collision, h_addr_zero⟩ | h_collision
+    simp at call_transfer
+    rcases call_transfer with ⟨s'_ok, transfer_right⟩
 
+    obtain ⟨s'_evm, ⟨s'_varstore, s'_all⟩⟩ := State_of_isOk s'_ok
 
+    have s9_ok : s₉.isOk := by
+      aesop
 
+    unfold reviveJump at code
+    simp [s'_all, ←s0_all] at code
+    rw [← State.insert_of_ok] at code
 
-    have h : ∀ {erc20 : ERC20}, IsERC20 erc20 s ∧ isEVMState s.evm →  preservesEvm s s' := by sorry
+    have s9_preserved : Preserved s'_evm s'_evm := by aesop
+    have s9_preservesEvm : preservesEvm s' s₉ := by
+      rw [s'_all, ←code]
+      apply s9_preserved
 
+    specialize transfer_right s_isERC20 isEvmState_s s_not_reverted
 
+    obtain ⟨s'_erc20, s'_preservesEvm, s'_not_reverted, s'_no_collision⟩
+              | ⟨s'_erc20, s'_preservesEvm, s'_no_collision, addr_balance_error, s'_reverted⟩
+              | s'_collision
+              := transfer_right
 
+    · rw [←code]
+      simp
+      have : s.evm.hash_collision = true → s'.evm.hash_collision = true := by
+        have account_map_preservation := (preservesEvm_of_isOk s_ok s'_ok s'_preservesEvm).2.1
+        aesop
+      aesop
 
-  · -- Hash collision at state s
-    sorry
+    · rw [←code]
+      simp
+      have : s.evm.hash_collision = true → s'.evm.hash_collision = true := by
+        have account_map_preservation := (preservesEvm_of_isOk s_ok s'_ok s'_preservesEvm).2.1
+        aesop
+      aesop
 
-    #exit
-
-
-
-
-
-
-    -- Want preservesEvm s0 s
-    -- then IsERC20 erc20 s0 --> IsERC20 erc20 s using IsERC20_of_preservesEvm
-    -- Problem is we have preservesEvm (Ok s0_evm Inhabited.default⟦"var_value"↦var_value⟧⟦"var_to"↦var_to⟧) s
-    -- Something to do with match in msgSender?
-    -- By preservesEVM definition, varstore variable is irrelevant
-    -- So substitute Inhabited.default for s0_varstore?
-
-    -- preserves s_inhabited s --> preserves s0 s
-    have s0inhabited_preserveEvm : preservesEvm (Ok s0_evm s0_varstore) (Ok s0_evm Inhabited.default⟦"var_value"↦var_value⟧⟦"var_to"↦var_to⟧) := by
-      exact Clear.Preserved.refl
-
-    have : preservesEvm (Ok s0_evm s0_varstore) s := by
-      exact Clear.Utilities.preservesEvm_trans  s_preservesEvm
-
-
-
-    -- preservesEvm s0 s → IsERC20 erc20 s0 → IsERC20 erc20 s₁
-
-    have : preservesEvm (Ok s0_evm s0_varstore) s_inhabited := by
-      dsimp [s_inhabited]
-      rw [preservesEvm_of_insert']
-      rw [preservesEvm_of_insert']
-      rcases s_inhabited with ⟨s_inhabited_evm, s_inhabited_varstore⟩
-      · simp
-      · simp
-      · simp
-
-    have : IsERC20 erc_20
-
-    have : ∀ {erc20 : ERC20}, IsERC20 erc20 s ∧ isEVMState s.evm →  preservesEvm s s' := by
-      specialize call_transfer ⟨is_erc20, s_preserve_evmState⟩
-      exact call_transfer.1
-
-    obtain ⟨erc20, ⟩ := call_transfer
-
-
-
-  #exit
-
-  -- assms
-  intro erc_20 is_erc20 evmState notReverted
-
-  obtain ⟨s_evm, s_varstore, s_ok⟩ := State_of_isOk s_isOk
-
-  -- get underlying Preserved from preservesEVM
-  rw [ s_ok, preservesEvm_of_insert, preservesEvm_of_insert ] at s_preservesEvm
-  have Preserved := Preserved_of_preservesEvm_of_Ok s_preservesEvm
-
-
-
-
-
-
-
-
-  /- rcases mapping with ⟨
-    ⟨preservesEvm, s_isOk, s_isEVMStatePreserved,
-    ⟨⟨keccak_value, keccak_using_keccak_value, hStore⟩,hHashCollision⟩⟩ | _, hHashCollision₁
-  ⟩ <;> [left; rcases s <;> aesop_spec] -/
-  #exit
-
-
-  -- refine' ⟨IsERC20_of_preservesEvm (by aesop) is_erc20, (by aesop), ?returns_correct_value⟩
-  refine' Or.inl ⟨?_, ?_, ?_, ?_, ?_⟩
-
-  · sorry
-
-
-
-  . -- Split on zero address case
-    by_cases h_recipient : (Address.ofUInt256 var_to).1 = 0
-    · -- Zero address case
-      right; left
-      -- Use refine to break up the conjunction into 6 subgoals
-      refine ⟨?_, ?_, ?_, ?_, ?_, ?_⟩
-
-      · apply IsERC20_of_preservesEvm ?_ isERC20
-        unfold preservesEvm
-        have : s₉.isOk := by
-          exfalso
-
-
-
-
-      -- Subgoal 1 - IsERC20 erc_20 s₉
-      -- Examining the structure of ISERC20 it has 5 parts which we refine into 5 subgoals
-      . refine ⟨?_, ?_, ?_, ?_, ?_⟩ -- #exit
-
-
-        -- Subsubgoal 1 - sload s₉.evm ERC20Private.totalSupply = erc_20.supply
-
-          -- We know that the total supply is the same as the initial supply at s₀
-        . have  s_0_supply : sload s₀.evm ERC20Private.totalSupply = erc_20.supply := by
-            dsimp [s₀] --unfold s₀ def
-            rcases isERC20 with ⟨h, _, _, _, _⟩ -- Unfold isERC20 but only extract the first field which is hasSupply into h
-            exact h
-
-          -- If we know this holds for s₀ then it must hold for s using mapping
-          have : sload s.evm ERC20Private.totalSupply = erc_20.supply := by
-            unfold A_fun_msgSender at mapping
-            unfold preservesEvm at mapping
-
-            match s with
-            | State.Ok evm' varstore' =>
-              have map_1 := mapping.1
-
-              have preserved_s : Preserved evm evm' := by
-                simp at map_1
-                exact map_1
-
-              have preserved_eq : sload s₀.evm ERC20Private.totalSupply = sload (State.Ok evm' varstore).evm ERC20Private.totalSupply := by
-                apply EVMState.sload_eq_of_preserved preserved_s
-
-              rw [s_0_supply] at preserved_eq
-              simp [preserved_eq]
-
-          -- If it holds for s then it holds for s' using mapping'
-          have : sload s'.evm ERC20Private.totalSupply = erc_20.supply := by
-            unfold A_fun__transfer at mapping'
-
-            -- Considering cases of A_fun__transfer we only need to look at the second case where address is 0
-            -- But we must show IsERC20 erc20 s ∧ isEVMState s.evm
-            -- from this we deduce preservesEVM s s'
-            -- Similar to above we can use lemma Preserved_of_preservesEvm_of_Ok to get the desired result
-
-          have : sload s₉.evm ERC20Private.totalSupply = erc_20.supply := by
-
-    . -- Non-zero address case -/
-      left
-      constructor
-      · sorry
-      . sorry
-
-
-
-
+    · aesop
 
 
 
